proof/refine/ARM/Finalise_R.thy
@@ -2910,7 +2910,9 @@ lemma replyUnlink_st_tcb_at_simplish:
   "replyUnlink r \<lbrace>st_tcb_at' (\<lambda>st. P st \<or> simple' st) t\<rbrace>"
   supply if_split [split del]
   unfolding replyUnlink_def
-  by (wpsimp wp: sts_st_tcb' hoare_vcg_if_lift2 hoare_vcg_imp_lift' simp: getReplyTCB_def)
+  apply (wpsimp wp: sts_st_tcb' hoare_vcg_if_lift2 hoare_vcg_imp_lift' gts_wp'
+              simp: getReplyTCB_def)
+  done
 
 crunch st_tcb_at_simplish: cteDeleteOne
             "st_tcb_at' (\<lambda>st. P st \<or> simple' st) t"
